src/coq/optimisations/add_instr.v
@@ -1,18 +1,27 @@
 
 Require Import ZArith.
 Require Import List.
-
+Require Import String Ascii.
 Require Import Bool.
 Require Import ZArith.Int.
 Require Import Vellvm.CFG.
 Require Import Vellvm.Ollvm_ast.
-Require Import Vellvm.optimisations.transform.
+Require Import Vellvm.Classes.
 Require Import ZArith List String Omega.
 Require Import Vellvm.AstLib Vellvm.Ollvm_ast.
+Require Import Vellvm.optimisations.wellformedSSA.
+Require Import Vellvm.optimisations.EqNat.
 
+From mathcomp.ssreflect
+Require Import ssreflect ssrbool seq eqtype ssrnat fintype.
+
+
+
+Require Import Equalities.
 Import ListNotations.
 Print instr_id.
 Print raw_id.
+
 
 
 (*Instr_id is of type raw_id*)
@@ -35,6 +44,7 @@ match c with
 end.
 
 
+
 (*So that an instruction with a unique UID can be added, we need to find to find an unused value*)
 Print block.
 Print instr_id.
@@ -44,13 +54,106 @@ match b.(blk_term) with
   | (_, _) => Z0
 end.
 
+
 (*Find the largest instruction (which is either the terminator ID or an instruction from within the code) and adds 1 to it*)
 Definition get_first_unused (b:block) : instr_id := IId (Raw (Z.add (get_maximum (get_terminator_iid b) (b.(blk_code))) 1)).
 
 (*Useless instruction*)
 Definition no_instr : instr := INSTR_Op (SV (VALUE_Null)).
+Print block.
+
+Definition optimise_block (b:block) := mk_block b.(blk_id) b.(blk_phis) (b.(blk_code)++[::(get_first_unused b, no_instr)]) b.(blk_term).
 
 
+Print uniq.
+Print instr_id_eqType.
+
+Lemma remove_nil_l : forall (a: seq instr_id), a = [::] ++ a.
+Proof. move => //a. Qed.
+
+Lemma remove_nil_r : forall (a: seq instr_id), a = a ++ [::].
+Proof. move => //a. induction a. simpl. auto. simpl. rewrite <- IHa. auto. Qed.
+
+
+Lemma instr_id_comm : forall (a b:instr_id), (a == b) = (b == a).
+Proof. intros. induction a, b => //. Qed.
+
+Lemma uniq_comm_single : forall (a b:instr_id), uniq ([::a] ++ [::b]) = uniq ([::b] ++ [::a]).
+Proof. intros. unfold uniq. simpl. unfold negb. unfold in_mem. simpl. rewrite instr_id_comm. auto.
+Qed.  
+
+
+
+
+Lemma notin_assoc : forall (a b c:instr_id), (a \notin ([::b] ++ [::c])) = ((a \notin [::b]) && (a \notin [::c])).
+Proof. move => //a b c. unfold negb. unfold in_mem. simpl. destruct (a == b) => //; destruct (a == c) => //.
+Qed.
+
+Lemma in_nil : forall (a:instr_id), (a \in [::]) = false.
+Proof. intros. unfold in_mem. simpl. auto. Qed.
+
+
+Lemma in_assoc : forall (a b:instr_id) (c:seq instr_id), (a \in ([::b] ++ c)) = (a \in [::b]) || (a \in c).
+Proof. intros. simpl. induction c => //.
+  +simpl. rewrite in_nil => //. rewrite orb_false_r. auto.
+  +simpl. unfold in_mem in *. simpl in *. destruct ((a == b)). simpl in *. auto.
+simpl in *. destruct ((a == a0)). simpl. auto. simpl. auto. Qed.
+
+
+
+Lemma in_assoc_list : forall (a:instr_id) (b c:seq instr_id), (a \in (b ++ c)) = (a \in b) || (a \in c).
+Proof. move => a b c. induction b, c => //.
+  +simpl. rewrite <- remove_nil_r. rewrite in_nil. rewrite orb_false_r. auto.
+  +simpl in *. unfold in_mem in *. simpl in *. destruct (a == a0) => //. Qed.
+
+
+Lemma in_assoc_r : forall a (b:seq instr_id) i, (i \in b ++ [:: a]) = (i \in b) || (i \in [:: a]).
+Proof. intros. rewrite in_assoc_list. auto. Qed.
+
+
+Lemma notin_assoc_one_list : forall (a b:instr_id) c, (a \notin ([::b] ++ c)) = ((a \notin [::b]) && (a \notin c)).
+Proof. intros. unfold negb. induction c => //.
+  +simpl. rewrite andb_true_r. auto.
+  +simpl in *. unfold in_mem in *. simpl in *. destruct (a == b) => //. Qed.
+
+
+
+Lemma notin : forall (a b:instr_id) (c:seq instr_id), (a \notin ([::b] ++ c) = (a \notin (c ++ [::b]))).
+Proof. intros. unfold negb. simpl. induction c => //.
+  +unfold in_mem. simpl. destruct (a == a0). destruct (a == b). simpl. auto. simpl. auto. rewrite IHc. simpl.
+unfold in_mem. simpl. auto. Qed.
+(*
+Lemma single_in_eq : forall (a i:instr_id), (i \in [:: a]) = (i == a).
+Proof. intros. unfold in_mem. simpl. auto. destruct ((i == a)) => //.
+Qed.
+Lemma testtest : forall (a:instr_id) (b:seq instr_id),  (a \notin b) && uniq b = uniq (b ++ [::a]).
+Proof. move => a b => //. induction b.
+  +simpl. auto.
+  +simpl. rewrite <- IHb. unfold negb. simpl. rewrite in_assoc_r. rewrite in_assoc. simpl.
+rewrite single_in_eq. rewrite single_in_eq. rewrite instr_id_comm. unfold in_mem. remember ((mem b) a) as B.
+destruct b; simpl => //. simpl. destruct (a0 == a). simpl. auto. simpl. auto.
+simpl. destruct (a == i). simpl. destruct (a0 == i). destruct (a0 == a). simpl. auto.
+simpl. auto.
+destruct (a0 == a). destruct (b a0).
+
+
+
+
+Lemma add_instr_preserves_ssa : forall b, well_form_block b -> well_form_block (optimise_block b).
+Proof. move =>// b. constructor. inversion H. unfold unique_instr_id in *. rewrite /optimise_block/=. 
+assert (([seq fst i
+      | i <- blk_code b ++
+             [:: (get_first_unused b, no_instr)]]) = [seq fst i
+      | i <- blk_code b] ++ [::fst (get_first_unused b, no_instr)]) => //. destruct b. simpl in *. induction blk_code => //. simpl.
+apply IHblk_code in H.
+
+
+Admitted.
+
+
+
+*)
+(*
 
 (*The code in a block gets executed sequentially.
 This optimisation adds an instruction to the end of that code therefore the impact this might have is on the block terminator instruction.
@@ -77,56 +180,10 @@ Let's add an instruction to a block if and only if its terminating instruction i
 (*Simple function that returns true if the terminating instruction is a return void*)
 Definition terminator_check (b:block) : bool :=
 match b.(blk_term) with
-  | (_, TERM_Ret_void) => true
+  | (_, TERM_Ret_void) => false
   | _ => false
 end.
 
-Print block.
-Print block.
-Print fetch.
-Locate fetch.
-Print block_to_cmd.
-Print block.
-
-
-Definition fetch_two_block (b1: block) (c:code) (i:instr_id) : option (cmd * option instr_id) :=
-match block_to_cmd b1 i with
-  | None => match block_to_cmd (mk_block b1.(blk_id) b1.(blk_phis) c b1.(blk_term)) i with
-            | None => None
-            | Some t => Some t
-            end
-(*If terminator => test*)
-(*If new => test*)
-  | Some a => Some a
-end.
-
-
-
-
-(*
-Definition fetch (CFG : mcfg) (p:pc) : option cmd :=
-  let 'mk_pc fid bid iid := p in 
-  'cfg <- find_function CFG fid;
-  'blk <- find_block (blks (df_instrs cfg)) bid;
-  '(c, _) <- block_to_cmd blk iid;
-  mret c.*)
-
-
-(*
-
-We want something like
-  let 'mk_pc fid bid iid := p in 
-  'cfg <- find_function CFG fid;
-  'blk <- find_block (blks (df_instrs cfg)) bid;
-  '(c, _) <- dual_block_to_cmd blk i;
-  mret c.*)
-
-Print block.
-Print blk_code.
-
-Definition add_instr_block (b:block) (i:(instr_id * instr)) (b1:(instr_id * terminator)%type) := 
-mk_block b.(blk_id) b.(blk_phis) (blk_code b ++ (cons i nil)) b1.
-Print blk_term.
 
 Definition get_blk_id (b:block) : instr_id :=
 let term := b.(blk_term) in
@@ -134,16 +191,236 @@ match term with
   | (term_id, term_instr) => term_id
 end.
 
+Print block.
+
+
+
+Print block_to_cmd.
+Print fallthrough.
+
+
+
+Definition old (c:code) (p:instr_id) (term_id:instr_id) := find_instr c p term_id.
+
+
+Definition add_instr_block (b:block) (i:(instr_id * instr)) (b1:(instr_id * terminator)%type) := 
+mk_block b.(blk_id) b.(blk_phis) (blk_code b ++ (cons i nil)) b1.
+Print blk_term.
+
 Definition get_blk_term (b:block)  :=
 let term := b.(blk_term) in
 match term with 
   | (term_id, term_instr) => term_instr
 end.
 
-(*V1*)
+Print block.
+
+
+
+
+
+(*Definition fallthrough (cd: code) term_id : instr_id :=
+  match cd with
+  | [] => term_id
+  | (next, _)::_ => next
+  end.*)
+
+
+
+
 Print block_to_cmd.
-(*The added instruction has the instruction id of the terminator instruction*)
-Definition optimisev1 (b:block) := if terminator_check b then (add_instr_block b (get_blk_id b, no_instr) (b.(blk_term))) else b.
+Print find_instr.
+
+
+
+(*
+Definition block_to_cmd (b:block) (iid:instr_id) : option (cmd * option instr_id) :=
+  let term_id := blk_term_id b in 
+  if term_id == iid then
+    Some (Term (snd (blk_term b)), None)
+  else
+    find_instr (blk_code b) iid term_id 
+.
+
+
+Fixpoint find_instr (cd : code) (p:instr_id) (t:instr_id) : option (cmd * option instr_id) :=
+  match cd with
+  | [] =>  None
+  | (x,i)::cd =>
+    if p == x then
+      Some (Step i, Some (fallthrough cd t))
+    else
+      find_instr cd p t
+  end.
+
+
+*)
+
+
+Lemma test : forall c d look term, find_instr (c ++ d) look term = find_instr (c ++ d) look term.
+Proof. Admitted.
+
+Definition beq_ascii (a1 a2 : ascii) :=
+  match a1, a2 with
+  | Ascii b1 b2 b3 b4 b5 b6 b7 b8, Ascii c1 c2 c3 c4 c5 c6 c7 c8 =>
+    (eqb b1 c1) && (eqb b2 c2) && (eqb b3 c3) && (eqb b4 c4) &&
+    (eqb b5 c5) && (eqb b6 c6) && (eqb b7 c7) && (eqb b8 c8)
+  end.
+
+
+Fixpoint beq_string (s1 s2 : string) :=
+  match s1, s2 with
+  | EmptyString,  EmptyString  => true
+  | String x1 s1, String x2 s2 => beq_ascii x1 x2 && beq_string s1 s2
+  | _, _                       => false
+  end.
+
+
+Print raw_id.
+Print int.
+Definition beq_raw_id (a b: raw_id) : bool:=
+match a, b with
+  | Name a, Name b => beq_string a b
+  | Anon a, Anon b => Z.eqb a b
+  | Raw a, Raw b => Z.eqb a b
+  | _, _ => false
+end.
+Print instr_id.
+
+
+
+Definition beq_instr_id (a b: instr_id) : bool:=
+match a, b with
+  | IId a, IId b => beq_raw_id a b
+  | IVoid a, IVoid b => Z.eqb a b
+  | _, _ => false
+end.
+
+
+Lemma ascii_eq : forall a, beq_ascii a a = true.
+Proof. intros a. induction a. simpl.
+repeat (rewrite eqb_reflx; simpl). auto. Qed.
+
+Lemma string_eq : forall s, beq_string s s = true.
+Proof. intros. induction s.
+  -simpl. auto.
+  -simpl. rewrite ascii_eq. simpl. rewrite IHs. auto. Qed.
+
+
+
+
+Lemma raw_id_eq : forall a, beq_raw_id a a = true.
+Proof. intros. induction a; simpl; try (rewrite string_eq); try (rewrite Z.eqb_refl); auto.
+Qed.
+
+Lemma instr_id_eq : forall a, beq_instr_id a a = true.
+Proof. intros. induction a; simpl; try (rewrite raw_id_eq); try (rewrite Z.eqb_refl); auto.
+Qed.
+
+Print fallthrough.
+(*Definition fallthrough (cd: code) term_id : instr_id :=
+  match cd with
+  | [] => term_id
+  | (next, _)::_ => next
+  end.*)
+
+
+Definition double_fallthrough (c d: code) (term_id:instr_id) : instr_id :=
+match c with
+  | [] => fallthrough d term_id
+  | _ => fallthrough c term_id
+end.
+
+Lemma double_fallthrough_eq : forall c d term_id, fallthrough (c ++ d) term_id = double_fallthrough c d term_id.
+Proof. intros. unfold double_fallthrough. unfold fallthrough.
+simpl. destruct c; simpl.
+  +simpl. auto.
+  +destruct p. auto.
+Qed.
+
+
+Print block_to_cmd.
+
+
+(*Fixpoint find_instr (cd : code) (p:instr_id) (t:instr_id) : option (cmd * option instr_id) :=
+  match cd with
+  | [] =>  None
+  | (x,i)::cd =>
+    if p == x then
+      Some (Step i, Some (fallthrough cd t))
+    else
+      find_instr cd p t
+  end.*)
+
+
+
+Definition double_find_instr (c d: code) (p :instr_id) (t:instr_id) : option (cmd * option instr_id) :=
+match (find_instr c p t) with
+  | None => (find_instr d p t)
+  | Some (Step i, Some ter) => if beq_instr_id ter t then Some (Step i, Some (fallthrough d t)) else Some (Step i, Some ter)
+  | Some (_, _) => find_instr d p t
+end.
+
+(*
+Lemma help : forall t, (fallthrough [] t) = t.
+Proof. intros. unfold fallthrough; simpl; eauto.
+Qed.
+
+Lemma help1 : forall p t, find_instr [] p t = None.
+Proof. intros. unfold find_instr. auto. Qed.
+
+
+Lemma help2: forall a d p t, find_instr (a::d) p t = double_find_instr (cons a nil) d p t.
+Proof. intros. induction a. simpl. unfold double_find_instr.
+simpl. destruct (p == a ). simpl.
+rewrite instr_id_eq. auto. auto. Qed.
+(* (fallthrough (c ++ d) t))*)
+
+
+
+
+
+Lemma test12 : forall c d p t, find_instr (c ++ d) p t = double_find_instr c d p t.
+Proof. intros.
+unfold double_find_instr. simpl.
+induction c.
+  +simpl. auto.
+  +rewrite help2. 
+assert (((a :: c) ++ d) = cons a (c ++ d)).
+simpl; auto. rewrite H. rewrite help2. 
+unfold double_find_instr. rewrite IHc.
+simpl. destruct a. simpl.
+
+Definition optimise (b:block) := if terminator_check b then (add_instr_block b (get_blk_id b, no_instr) (get_first_unused b, get_blk_term b)) else b.
+
+Definition prog_optimise (p:modul CFG.cfg) := def_cfg_opt optimise p.
+
+(*
+(*V1*)
+(*Get new instructions*)
+
+(*Proof: block_to_cmd (optimise b) p = fetch_two_block b (optimise b) (new:code) p*)
+
+
+
+Definition fetch_two_block_full  (b:block) (p:instr_id) :=
+if terminator_check b then (fetch_two_block b (optimisev1 b) (cons (get_first_unused b, no_instr) nil) p) else (block_to_cmd b p).
+
+
+Lemma block_eq : forall b p, block_to_cmd (optimisev1 b) p = fetch_two_block_full b p.
+Proof. intros. unfold block_to_cmd. unfold fetch_two_block_full. unfold optimisev1. 
+unfold terminator_check. destruct b. simpl. destruct blk_term. simpl. unfold blk_term_id. 
+unfold block_to_cmd. simpl. unfold fetch_two_block. simpl. unfold blk_term_id. simpl.
+destruct t; simpl; auto.
+  +unfold block_to_cmd. simpl. unfold blk_term_id. simpl. unfold get_first_unused. simpl.
+destruct (i == p). auto.
+  *destruct blk_code. simpl. unfold get_terminator_iid. simpl. unfold not in n.
+induction i; simpl; auto. induction id. simpl.
+
+Require Import Vellvm.optimisations.transform. 
+
+
+Definition optimise_addv1 (b:block) := if terminator_check b then cons (get_first_unused b, no_instr) nil else nil.
 
 Definition prog_optimisev1 (p:modul CFG.cfg) := def_cfg_opt optimisev1 p.
 
@@ -155,12 +432,21 @@ Definition prog_optimisev1 (p:modul CFG.cfg) := def_cfg_opt optimisev1 p.
 As seen in the pacoproof.v, it is useful to write (fetch (optimise prog) pc) as a new function of fetch prog pc.
 This allows us to 
 *)
-(*V2*)
+(*V2*)(*
+Definition optimisev2 (b:block) := if terminator_check b then (add_instr_block b (get_blk_id b, no_instr) (
+*)
+Print block_to_cmd.
+
+
+
+
+Print find_instr.
+Print block_to_cmd.
 
 
 
 (**************************************************************************)
-Definition dual_block_to_cmd (b:block) (i:instr_id) := if terminator_check b then fetch_two_block b (cons (get_blk_id b, no_instr) nil) i else block_to_cmd b i .
+Definition dual_block_to_cmd (b:block) (i:instr_id) := if terminator_check b then fetch_two_block b (cons (get_first_unused b, no_instr) nil) i else block_to_cmd b i .
 
 
 Require Import Vellvm.Classes.
@@ -174,28 +460,24 @@ Definition dual_fetch (CFG: mcfg) (p:pc) :=
 
 
 Lemma test1 : forall b i, dual_block_to_cmd b i = block_to_cmd (optimisev1 b) i.
-Proof. intros. unfold dual_block_to_cmd. unfold optimisev1.
-unfold terminator_check. destruct b. simpl in *. destruct blk_term.
-destruct t; auto. 
-  +unfold fetch_two_block. simpl in *.
-unfold add_instr_block. simpl in *.
-remember ([(get_blk_id
-                        {|
-                        blk_id := blk_id;
-                        blk_phis := blk_phis;
-                        blk_code := blk_code;
-                        blk_term := (i0, TERM_Ret_void) |}, no_instr)]) as A.
-
-
-unfold block_to_cmd. simpl. unfold blk_term_id. simpl.
-simpl.
-induction (i0 == i). auto. subst. simpl. unfold get_blk_id. simpl.
-induction blk_code. simpl. unfold not in b. simpl in *.
-destruct (i == i0). symmetry in e. apply b in e. inversion e. auto.
-simpl. destruct a.
-destruct (i == i1). simpl.
--unfold fallthrough. simpl. destruct blk_code. simpl. auto. simpl. auto.
--auto.
+Proof. intros. unfold dual_block_to_cmd. unfold terminator_check.
+destruct b. simpl. unfold optimisev1. simpl. unfold get_first_unused. simpl. destruct blk_term.
+simpl. destruct t; simpl; auto.
+  -unfold fetch_two_block. simpl. unfold block_to_cmd. simpl. unfold blk_term_id.
+simpl. unfold get_terminator_iid. simpl. destruct (i0 == i); auto.
+induction blk_code. simpl. auto.
+remember (i ==
+    IId
+      (Raw
+         (match i0 with
+          | IId (Name _) => 0
+          | IId (Anon _) => 0
+          | IId (Raw n0) => n0
+          | IVoid _ => 0
+          end + 1)%Z)) as A. destruct A; auto. simpl. destruct a. simpl.
+destruct (i == i1). simpl. unfold fallthrough. simpl.
+destruct blk_code. simpl. unfold not in n. destruct i1. simpl. destruct id. simpl.
+destruct i0. destruct id; simpl. simpl in *.
 Qed.
 
 
@@ -298,8 +580,8 @@ simpl. destruct blk_code; simpl; auto.
 }
   +auto.
 }
-Qed.
+Qed.*)
 
-
-
+*)
+*)
 (**************************************************************************)
